date: 08.18.2022
tags: #physics/mechanics/motion  
# Constant Angular Acceleration
These are the same equations for **constant linear acceleration**, and respective variables can just be substituted for the equations to work for this scenario:

Most fundamental equations (all others can be derived):
1. $$\omega = \omega_0 + \alpha t$$
2. $$\theta - \theta_0 = \omega_0t+\frac{1}{2}\alpha t^2$$

Derived equations:

3. $$\omega^2 = \omega_0^2 + 2\alpha (\theta-\theta_0)$$
4. $$\theta - \theta_0 = \frac{1}{2}(\omega_0 + \omega)t$$
5. $$\theta - \theta_0 = \omega t - \frac{1}{2}\alpha t^2$$